sha/spec_hmac.v
@@ -57,12 +57,12 @@ Definition absCtxt (h:hmacabs): s256abs :=
   match h with HMACabs ctx _ _ _ _ => ctx end.
 
 Definition innerShaInit (k: list byte) (s:s256abs):Prop :=
-  update_abs (HMAC_SHA256.mkArgZ k Ipad) init_s256abs s.
+  update_abs (HP.HMAC_SHA256.mkArgZ k HP.Ipad) init_s256abs s.
 Definition outerShaInit (k: list byte) (s:s256abs):Prop :=
-  update_abs (HMAC_SHA256.mkArgZ k Opad) init_s256abs s.
+  update_abs (HP.HMAC_SHA256.mkArgZ k HP.Opad) init_s256abs s.
 
 Definition hmacInit (k:list Z) (h:hmacabs):Prop :=  
-  let key := HMAC_SHA256.mkKey k in
+  let key := HP.HMAC_SHA256.mkKey k in
   let keyB := map Byte.repr key in
   exists iS oS, innerShaInit keyB iS /\ outerShaInit keyB oS /\
   h = HMACabs iS iS oS (if zlt 64 (Zlength k) then 32 else Zlength k) k.
@@ -106,7 +106,7 @@ Definition hmacSimple (k:list Z) (data:list Z) (dig:list Z) :=
 
 Lemma hmacSimple_sound k data dig: 
       hmacSimple k data dig ->
-      dig = HMAC256 data k.
+      dig = HP.HMAC256 data k.
 Proof.
  unfold hmacSimple; intros [hInit [hUpd [HH1 [HH2 HH3]]]].
  unfold hmacInit in HH1. destruct HH1 as [iInit [oInit [HiInit [HoInit HINIT]]]]. subst.
@@ -114,15 +114,16 @@ Proof.
    rewrite Zlength_correct in *; simpl in *. subst.
  unfold outerShaInit in HoInit. inversion HoInit; clear HoInit.
    rewrite Zlength_correct in *; simpl in *. subst.
- unfold HMAC_SHA256.mkArgZ in *.
+ unfold HP.HMAC_SHA256.mkArgZ in *.
  destruct HH2 as [ctx2 [Hupd HU]]. subst.
  inversion Hupd; clear Hupd. subst.
  unfold hmacFinalSimple in HH3. destruct HH3 as [oS [Upd FINISH]]. subst.
  inversion Upd; clear Upd. subst.
- unfold HMAC256, HMAC_SHA256.HMAC, HMAC_SHA256.OUTER, HMAC_SHA256.INNER.
- unfold sha_finish. unfold SHA256.Hash. rewrite functional_prog.SHA_256'_eq. f_equal.
- unfold HMAC_SHA256.innerArg, HMAC_SHA256.mkArgZ. rewrite H7. clear H7. 
- unfold HMAC_SHA256.outerArg, HMAC_SHA256.mkArgZ. rewrite H12. clear H12.
+ unfold HP.HMAC256, HP.HMAC_SHA256.HMAC, HP.HMAC_SHA256.HmacCore, HP.HMAC_SHA256.KeyPreparation, HP.HMAC_SHA256.OUTER, HP.HMAC_SHA256.INNER.
+ unfold sha_finish. unfold HP.SHA256.Hash.
+ rewrite functional_prog.SHA_256'_eq. f_equal.
+ unfold HP.HMAC_SHA256.innerArg, HP.HMAC_SHA256.mkArgZ. rewrite H7. clear H7. 
+ unfold HP.HMAC_SHA256.outerArg, HP.HMAC_SHA256.mkArgZ. rewrite H12. clear H12.
  unfold sha_finish in *. rewrite intlist_to_Zlist_app in *.
 rewrite <- app_assoc. rewrite <- H22; clear H22. 
 repeat rewrite <- app_assoc. rewrite H17. reflexivity. 
@@ -159,7 +160,7 @@ Qed.
 
 Lemma hmac_sound k data dig h: 
       hmac k data dig h ->
-      dig = HMAC256 data k.
+      dig = HP.HMAC256 data k.
 Proof.
  intros.
  eapply hmacSimple_sound.
@@ -196,7 +197,7 @@ Definition hmac_relate (h: hmacabs) (r: hmacstate) : Prop :=
     s256_relate iS (iCtx r) /\
     s256_relate oS (oCtx r) /\
     s256a_len iS = 512 /\ s256a_len oS = 512 /\ 
-    Key r = map Vint (map Int.repr (HMAC_SHA256.mkKey k)) /\ 
+    Key r = map Vint (map Int.repr (HP.HMAC_SHA256.mkKey k)) /\ 
     exists i, Keylen r = Vint i /\ klen=Int.unsigned i /\ 
               (if zlt 64 (Zlength k) then 32 else Zlength k)=klen
   end.
@@ -235,10 +236,10 @@ Definition hmac_relate_PreInitNull (key:list Z) (h:hmacabs ) (r: hmacstate) : Pr
     s256_relate iS (iCtx r) /\
     s256_relate oS (oCtx r) /\
     s256a_len iS = 512 /\ s256a_len oS = 512 /\ 
-    Key r = map Vint (map Int.repr (HMAC_SHA256.mkKey k)) /\ 
+    Key r = map Vint (map Int.repr (HP.HMAC_SHA256.mkKey k)) /\ 
     exists i, Keylen r = Vint i /\ klen=Int.unsigned i /\ 
               (if zlt 64 (Zlength k) then 32 else Zlength k)=klen /\
-    let keyB := map Byte.repr (HMAC_SHA256.mkKey key) in
+    let keyB := map Byte.repr (HP.HMAC_SHA256.mkKey key) in
     innerShaInit keyB iS /\ outerShaInit keyB oS
   end.
 
@@ -319,7 +320,7 @@ Definition hmac_relate_PostFinal (h:hmacabs ) (r: hmacstate) : Prop :=
     s256_relate iS (iCtx r) /\
     s256_relate oS (oCtx r) /\
     s256a_len iS = 512 /\ s256a_len oS = 512 /\ 
-    Key r = map Vint (map Int.repr (HMAC_SHA256.mkKey k)) /\ 
+    Key r = map Vint (map Int.repr (HP.HMAC_SHA256.mkKey k)) /\ 
     exists i, Keylen r = Vint i /\ klen=Int.unsigned i /\ 
               (if zlt 64 (Zlength k) then 32 else Zlength k)=klen
   end.
@@ -410,7 +411,7 @@ Definition HMAC_spec :=
              `(memory_block shmd (Int.repr 32) md))
   POST [ tvoid ] 
          EX digest:_, 
-          PROP (digest = HMAC256 (CONT MSG) (CONT KEY))
+          PROP (digest = HP.HMAC256 (CONT MSG) (CONT KEY))
           LOCAL ()
           SEP(`(K_vector KV);
               `(data_block shmd digest md);
@@ -475,7 +476,7 @@ Definition HMAC_Double_spec :=
              `(memory_block shmd (Int.repr 64) md))
   POST [ tvoid ] 
          EX digest:_, 
-          PROP (digest = HMAC256 (CONT MSG) (CONT KEY))
+          PROP (digest = HP.HMAC256 (CONT MSG) (CONT KEY))
           LOCAL ()
           SEP(`(K_vector KV);
               `(data_block shmd (digest++digest) md);
@@ -527,4 +528,4 @@ Definition emptySha:s256state := (nil, (Vundef, (Vundef, (nil, Vundef)))).
 Definition keyedHMS key: hmacstate :=
   (emptySha, (emptySha, (emptySha, 
    (if zlt 64 (Zlength key) then Vint (Int.repr 32) else Vint (Int.repr (Zlength key)), 
-   map Vint (map Int.repr (HMAC_SHA256.mkKey key)))))).
+   map Vint (map Int.repr (HP.HMAC_SHA256.mkKey key)))))).
