sha/verif_hmacADT_double.v
@@ -331,10 +331,10 @@ apply andp_right. apply prop_right. split; trivial.
 apply andp_right. apply prop_right. trivial. cancel.
 rewrite sepcon_assoc. rewrite sepcon_comm.
 apply sepcon_derives.
-  assert (D1: dig = HMAC256 data key).
+  assert (D1: dig = HP.HMAC256 data key).
      apply hmac_sound with (h:=h2).
      exists h0, h1. auto.
-  assert (D2: dig2 = HMAC256 data key).
+  assert (D2: dig2 = HP.HMAC256 data key).
      eapply hmac_sound with (h:=h5).
      exists h3, h4. auto.
 
